progress towards adequacy

theories/examples/lse_adequacy.v
@@ -12,7 +12,7 @@ From cap_machine.examples Require Import template_adequacy.
 Instance DisjointList_list_Addr : DisjointList (list Addr).
 Proof. exact (@disjoint_list_default _ _ app []). Defined.
 
-Import with_adv.
+Import with_adv_and_link.
 
 Class memory_layout `{MachineParameters} := {
   (* Code of f *)
@@ -23,10 +23,12 @@ Class memory_layout `{MachineParameters} := {
   f_region_start_offset: (f_region_start + 1)%a = Some f_start;
 
   (* adversary code *)
+  adv_region_start : Addr;
   adv_start : Addr;
   adv_end : Addr;
   adv_instrs : list Word;
   adv_size : (adv_start + (length adv_instrs) = Some adv_end)%a ;
+  adv_region_start_offset: (adv_region_start + 1)%a = Some adv_start;
 
   (* malloc routine *)
   malloc_start : Addr;
@@ -62,6 +64,12 @@ Class memory_layout `{MachineParameters} := {
   link_table_size :
     (link_table_start + 2)%a = Some link_table_end;
 
+  (* adversary link table *)
+  adv_link_table_start : Addr;
+  adv_link_table_end : Addr;
+  adv_link_table_size :
+    (adv_link_table_start + 1)%a = Some adv_link_table_end;
+
   (* failure flag *)
   fail_flag : Addr;
   fail_flag_next : Addr;
@@ -71,10 +79,11 @@ Class memory_layout `{MachineParameters} := {
   (* disjointness of all the regions above *)
   regions_disjoint :
     ## [
-        region_addrs adv_start adv_end;
-        region_addrs f_start f_end;
+        region_addrs adv_region_start adv_end;
+        region_addrs f_region_start f_end;
         [fail_flag];
         region_addrs link_table_start link_table_end;
+        region_addrs adv_link_table_start adv_link_table_end;
         region_addrs fail_start fail_end;
         region_addrs malloc_mem_start malloc_end;
         [malloc_memptr];
@@ -82,23 +91,78 @@ Class memory_layout `{MachineParameters} := {
        ]
 }.
 
-Definition mk_initial_memory `{memory_layout} : gmap Addr Word :=
-    mkregion f_start f_end (roe_instrs 0 1 r_adv)
-  ∪ mkregion adv_start adv_end adv_instrs
-  ∪ mkregion 
-
-
-Definition roe_prog `{MachineParameters} `{memory_layout} : prog :=
+Definition roe_prog `{memory_layout} : prog :=
   {| prog_start := f_start ;
      prog_end := f_end ;
      prog_instrs := (roe_instrs 0 1 r_adv) ;
      prog_size := f_size |}.
 
-Definition adv_prog `{MachineParameters} `{memory_layout} : prog :=
+Definition adv_prog `{memory_layout} : prog :=
   {| prog_start := adv_start ;
      prog_end := adv_end ;
      prog_instrs := adv_instrs ;
      prog_size := adv_size |}.
+
+(* MALLOC library entry *)
+Definition malloc_library_content `{memory_layout} : gmap Addr Word :=
+  (* code for the malloc subroutine *)
+  mkregion malloc_start malloc_memptr malloc_subroutine_instrs
+  (* Capability to malloc's memory pool, used by the malloc subroutine *)
+  ∪ list_to_map [(malloc_memptr, WCap RWX malloc_memptr malloc_end malloc_mem_start)]
+  (* Malloc's memory pool, initialized to zero *)
+  ∪ mkregion malloc_mem_start malloc_end (region_addrs_zeroes malloc_mem_start malloc_end).
+
+Definition lib_entry_malloc `{memory_layout} : lib_entry :=
+  {| lib_start := malloc_start ;
+     lib_end := malloc_end ;
+     lib_full_content := malloc_library_content |}.
+
+(* FAIL library entry *)
+Definition fail_library_content `{memory_layout} : gmap Addr Word :=
+  (* code for the failure subroutine *)
+  (* tail contains pointer to the "failure" flag, set to 1 by the routine *)
+  mkregion fail_start fail_end (assert_fail_instrs ++ [WCap RW fail_flag fail_flag_next fail_flag])
+  ∪ list_to_map [(fail_flag, WInt 0%Z)] (* failure flag, initially set to 0 *).
+
+Definition lib_entry_fail `{memory_layout} : lib_entry :=
+  {| lib_start := fail_start ;
+     lib_end := fail_end ;
+     lib_full_content := fail_library_content |}.
+
+(* full library *)
+Definition library `{memory_layout} : lib :=
+  {| priv_libs := [lib_entry_fail] ;
+     pub_libs := [lib_entry_malloc] |}.
+
+Program Definition roe_table `{memory_layout} : @tbl_priv roe_prog library :=
+  {| prog_lower_bound := f_region_start ;
+     tbl_start := link_table_start ;
+     tbl_end := link_table_end ;
+     tbl_size := link_table_size ;
+     tbl_prog_link := f_region_start_offset ;
+     tbl_disj := _
+  |}.
+Next Obligation.
+  intros. simpl.
+  pose proof (regions_disjoint) as Hdisjoint.
+  rewrite !disjoint_list_cons in Hdisjoint |- *. intros (?&?&?&?&?&?&?&?&?).
+  disjoint_map_to_list. set_solver.
+Qed.
+
+Program Definition adv_table `{memory_layout} : @tbl_pub adv_prog library :=
+  {| prog_lower_bound := adv_region_start ;
+     tbl_start := adv_link_table_start ;
+     tbl_end := adv_link_table_end ;
+     tbl_size := adv_link_table_size ;
+     tbl_prog_link := adv_region_start_offset ;
+     tbl_disj := _
+  |}.
+Next Obligation.
+  intros. simpl.
+  pose proof (regions_disjoint) as Hdisjoint.
+  rewrite !disjoint_list_cons in Hdisjoint |- *. intros (?&?&?&?&?&?&?&?&?).
+  disjoint_map_to_list. set_solver.
+Qed.
 
 
 Definition OK_invariant `{MachineParameters} `{memory_layout} (m : gmap Addr Word) : Prop :=
@@ -120,3 +184,172 @@ Definition flag_inv `{MachineParameters} `{memory_layout} : memory_inv :=
   {| minv := OK_invariant ;
      minv_dom := {[ fail_flag ]} ;
      minv_dom_correct := OK_dom_correct |}.
+
+(* TODO: move to iris extra *)
+Lemma big_sepM_to_big_sepL2 (PROP : bi) (A B : Type) `{EqDecision A} `{Countable A}
+      (φ: A -> B -> PROP) (l1: list A) (l2: list B):
+      NoDup l1 -> length l1 = length l2 →
+      ⊢ (([∗ map] y1↦y2 ∈ list_to_map (zip l1 l2), φ y1 y2) -∗
+         ([∗ list] y1;y2 ∈ l1;l2, φ y1 y2))%I.
+Proof.
+  revert l2. iInduction (l1) as [|x l1] "IH"; iIntros (l2 Hnd Hlen) "H".
+  - iSimpl. destruct l2;inversion Hlen. done.
+  - destruct l2;inversion Hlen. simpl.
+    inversion Hnd. subst.
+    iDestruct (big_sepM_insert with "H") as "[A B]".
+    + eapply not_elem_of_list_to_map.
+      rewrite fst_zip; auto. lia.
+    + iFrame. iApply ("IH" $! l2 H4 H1 with "B"); auto.
+Qed.
+
+Section roe_adequacy.
+  Context {Σ:gFunctors} {memg:memG Σ} {regg:regG Σ}
+          {nainv: logrel_na_invs Σ}
+          `{memlayout: memory_layout}.
+
+  Definition mallocN : namespace := nroot .@ "roe" .@ "malloc".
+
+  Lemma roe_correct :
+    Forall (λ w, is_cap w = false) adv_instrs →
+    let filtered_map := λ (m : gmap Addr Word), filter (fun '(a, _) => a ∉ minv_dom flag_inv) m in
+  (∀ rmap,
+      dom (gset RegName) rmap = all_registers_s ∖ {[ PC; r_adv ]} →
+      ⊢ inv invN (minv_sep flag_inv)
+        ∗ na_own logrel_nais ⊤
+        ∗ PC ↦ᵣ WCap RWX (prog_lower_bound roe_table) (prog_end roe_prog) (prog_start roe_prog)
+        ∗ r_adv ↦ᵣ WCap RWX (prog_lower_bound adv_table) (prog_end adv_prog) (prog_start adv_prog)
+        ∗ ([∗ map] r↦w ∈ rmap, r ↦ᵣ w ∗ ⌜is_cap w = false⌝)
+        (* P program and table *)
+        ∗ (prog_lower_bound roe_table) ↦ₐ (WCap RO (tbl_start roe_table) (tbl_end roe_table) (tbl_start roe_table))
+        ∗ ([∗ map] a↦w ∈ (tbl_region roe_table), a ↦ₐ w)
+        ∗ ([∗ map] a↦w ∈ (prog_region roe_prog), a ↦ₐ w)
+        (* Adv program and table *)
+        ∗ (prog_lower_bound adv_table) ↦ₐ (WCap RO (tbl_start adv_table) (tbl_end adv_table) (tbl_start adv_table))
+        ∗ ([∗ map] a↦w ∈ (tbl_region adv_table), a ↦ₐ w)
+        ∗ ([∗ map] a↦w ∈ (prog_region adv_prog), a ↦ₐ w)
+        (* filtered entries *)
+        ∗ ([∗ map] a↦w ∈ (lib_region (pub_libs library)), a ↦ₐ w)
+        ∗ ([∗ map] a↦w ∈ filtered_map (lib_region (priv_libs library)), a ↦ₐ w)
+
+        -∗ WP Seq (Instr Executable) {{ λ _, True }}).
+  Proof.
+    iIntros (Hints Hfilter rmap Hdom) "(#Hinv & Hown & HPC & Hr_adv & Hrmap & Hroe_link & Hroe_table & Hroe
+                                 & Hadv_link & Hadv_table & Hadv & Hpubs & Hprivs)".
+
+    iDestruct (big_sepM_sep with "Hrmap") as "[Hrmap #Hrmapvalid]".
+    simpl. rewrite !map_union_empty.
+
+    (* setting up read only example program *)
+    iAssert (roe (region_addrs f_start f_end) 0 1 r_adv) with "[Hroe] "as "Hroe".
+    { rewrite /roe /prog_region /= /mkregion.
+      iApply big_sepM_to_big_sepL2. apply region_addrs_NoDup.
+      pose proof f_size as Hsize.
+      rewrite region_addrs_length /region_size. solve_addr +Hsize.
+      iFrame. }
+
+    (* cleaning up the environment tables *)
+    rewrite /tbl_region /mkregion /=.
+    pose proof link_table_size as Hsize.
+    assert (is_Some (link_table_start + 1)%a) as [link_table_mid Hmid]. solve_addr+Hsize.
+    rewrite region_addrs_cons;[|solve_addr +Hsize].
+    rewrite Hmid /= region_addrs_single /=;[|solve_addr +Hmid Hsize].
+    pose proof adv_link_table_size as Hsize_adv.
+    rewrite region_addrs_single /=;[|solve_addr +Hsize_adv].
+    iDestruct (big_sepM_insert with "Hroe_table") as "[Hlink_table_start Hroe_table]".
+    { rewrite lookup_insert_ne//. solve_addr +Hmid. }
+    iDestruct (big_sepM_insert with "Hroe_table") as "[Hlink_table_mid _]";auto.
+    iDestruct (big_sepM_insert with "Hadv_table") as "[Hadv_link_table_start _]";auto.
+
+    (* allocate malloc invariant *)
+    iMod (na_inv_alloc logrel_nais ⊤ mallocN (malloc_inv malloc_start malloc_end)
+            with "[Hpubs]") as "#Hinv_malloc".
+    { iNext. rewrite /malloc_inv. iExists malloc_memptr, malloc_mem_start.
+      rewrite /malloc_library_content.
+      iDestruct (big_sepM_union with "Hpubs") as "[Hpubs Hinit]".
+      { pose proof (regions_disjoint) as Hdisjoint.
+        rewrite !disjoint_list_cons in Hdisjoint |- *. intros (?&?&?&?&?&?&?&?&?).
+        disjoint_map_to_list. set_solver. }
+      iDestruct (big_sepM_union with "Hpubs") as "[Hpubs Hmid]".
+      { pose proof (regions_disjoint) as Hdisjoint.
+        rewrite !disjoint_list_cons in Hdisjoint |- *. intros (?&?&?&?&?&?&?&?&?).
+        disjoint_map_to_list. set_solver. }
+      pose proof malloc_code_size as Hmalloc_size.
+      pose proof malloc_memptr_size as Hmalloc_memptr_size.
+      pose proof malloc_mem_size as Hmalloc_mem_size.
+      iSplitL "Hpubs".
+      iApply big_sepM_to_big_sepL2. apply region_addrs_NoDup.
+      rewrite region_addrs_length /region_size.  solve_addr +Hmalloc_size.
+      assert ((malloc_start ^+ length malloc_subroutine_instrs)%a = malloc_memptr) as ->
+      ;[solve_addr+Hmalloc_size|iFrame].
+      iSplit;[auto|]. iDestruct (big_sepM_insert with "Hmid") as "[$ _]";auto.
+      iSplit;[|iPureIntro;solve_addr+Hmalloc_size Hmalloc_memptr_size Hmalloc_mem_size].
+      iApply big_sepM_to_big_sepL2. apply region_addrs_NoDup.
+      rewrite region_addrs_length replicate_length /region_size. solve_addr +Hmalloc_mem_size. iFrame. }
+    iDestruct (simple_malloc_subroutine_valid with "[$Hinv_malloc]") as "#Hmalloc_val".
+
+    (* allocate adversary table *)
+    iMod (inv_alloc (logN .@ adv_link_table_start) ⊤ (interp_ref_inv adv_link_table_start interp)
+            with "[Hadv_link_table_start]") as "#Hadv_table_valid".
+    { iNext. iExists _. iFrame. auto. }
+
+    (* allocate validity of adversary *)
+    pose proof adv_size as Hadv_size'.
+    pose proof adv_region_start_offset as Hadv_region_offset.
+    iDestruct (big_sepM_to_big_sepL2 with "Hadv") as "Hadv /=". apply region_addrs_NoDup.
+    rewrite region_addrs_length /region_size /=. solve_addr+Hadv_size'.
+    iMod (region_inv_alloc _ (region_addrs adv_region_start adv_end) (_::adv_instrs) with "[Hadv Hadv_link]") as "#Hadv".
+    { rewrite (region_addrs_cons adv_region_start);[rewrite Hadv_region_offset /=|solve_addr +Hadv_region_offset Hadv_size'].
+      iFrame. iSplit.
+      { iApply fixpoint_interp1_eq. iSimpl. iClear "∗".
+        rewrite region_addrs_single// /=. iSplit;[|done].
+        iExists interp. iFrame "Hadv_table_valid". auto. }
+      iApply big_sepL2_sep. iFrame. iApply big_sepL2_to_big_sepL_r.
+      rewrite region_addrs_length /region_size /=. solve_addr+Hadv_size'.
+      iApply big_sepL_forall. iIntros (k n Hin).
+      revert Hints; rewrite Forall_forall =>Hints.
+      assert (n ∈ adv_instrs) as HH%Hints;[apply elem_of_list_lookup;eauto|]. destruct n;inversion HH.
+      iApply fixpoint_interp1_eq;eauto. }
+
+    iAssert (interp (WCap RWX adv_region_start adv_end adv_start)) as "#Hadv_valid".
+    { iClear "∗". iApply fixpoint_interp1_eq. iSimpl.
+      iDestruct (big_sepL2_to_big_sepL_l with "Hadv") as "Hadv'".
+      { rewrite region_addrs_length /region_size. solve_addr+Hadv_region_offset Hadv_size'. }
+      iApply (big_sepL_mono with "Hadv'").
+      iIntros (k y Hin) "Hint". iExists interp. iFrame. auto. }
+
+    iApply (roe_spec with "[- $HPC $Hown $Hr_adv $Hroe_link $Hrmap $Hroe $Hinv_malloc
+                              $Hlink_table_start $Hlink_table_mid $Hadv_valid]");auto.
+    instantiate (1:=f_end).
+    { intros mid Hmid'. split;auto. pose proof (f_region_start_offset) as HH. solve_addr+HH Hmid'. }
+    { apply contiguous_between_of_region_addrs;auto. pose proof (f_size) as HH. solve_addr+HH. }
+    { apply le_addr_withinBounds'. solve_addr+Hsize Hmid. }
+    { apply le_addr_withinBounds'. solve_addr+Hsize Hmid. }
+    { solve_addr. }
+
+    iApply (inv_iff with "Hinv []"). iNext. iModIntro.
+    iSplit.
+    - rewrite /minv_sep /=. iIntros "HH". iDestruct "HH" as (m) "(Hm & %Heq & %HOK)".
+      assert (is_Some (m !! fail_flag)) as [? Hlook].
+      { apply elem_of_gmap_dom. rewrite Heq. apply elem_of_singleton. auto. }
+      iDestruct (big_sepM_lookup _ _ fail_flag with "Hm") as "Hflag";eauto.
+      apply HOK in Hlook as ->. iFrame.
+    - iIntros "HH". iExists {[ fail_flag := WInt 0%Z ]}.
+      rewrite big_sepM_singleton. iFrame.
+      rewrite dom_singleton_L /minv_dom /=. iSplit;auto.
+      rewrite /OK_invariant. iPureIntro. intros w Hw. simplify_map_eq. done.
+  Qed.
+
+End roe_adequacy.
+
+Theorem template_adequacy `{memory_layout}
+    (m m': Mem) (reg reg': Reg) (es: list cap_lang.expr):
+  is_initial_memory roe_prog adv_prog library roe_table adv_table m →
+  is_initial_registers roe_prog adv_prog library roe_table adv_table reg r_adv →
+  Forall (λ w, is_cap w = false) (prog_instrs adv_prog) →
+
+  rtc erased_step ([Seq (Instr Executable)], (reg, m)) (es, (reg', m')) →
+  minv flag_inv m'.
+Proof.
+  intros ? ? Hints ?.
+  pose proof template_adequacy as Hadequacy. eapply Hadequacy;eauto.
+Admitted.
